Finished proving p2c

Distributed/Paxos/p2c.lean
@@ -4,36 +4,38 @@ import Distributed.Paxos.learner_helpers
 import Mathlib.Tactic.ByContra
 import Mathlib.Tactic.Cases
 
+
 open Model
 open PaxosModel
 namespace PaxosProof
 
 
 
-def inv4c4 (s: System a l p) (i: Fin p) (j: Fin a) :=
-(s.proposers i).propRec j = true
--> (Message.Promise (s.proposers i).propId j none ∈ s.network.messages ∨ ∃ v, (s.proposers i).propVal = some v)
 
 
 --INV4c1
 def inv4c1 (s: System a l p) (i: Fin p) :=
 (s.proposers i).propVal = none
--> ∀ j, contains (s.proposers i).propRec j = true
--> Message.Promise (s.proposers i).propId j none ∈ s.network.messages
+-> (∀ j, contains (s.proposers i).propRec j = true
+-> Message.Promise (s.proposers i).propId j none ∈ s.network.messages)
+∧ (s.proposers i).accPropId = 0
 
 
 theorem inv4c1Proof_ind (s1 s2: System a l p) (i: Fin p):
 step s1 s2
 -> inv4c1 s1 i
 -> inv4c1 s2 i := by
-simp [inv4c1]; intros step IH sPropNone j jContained
+simp [inv4c1]; intros step IH sPropNone 
 cases step <;> rename_i stepRule <;> cases stepRule <;> repeat (rename_i stepRule; rcases stepRule) <;> (try simp [updateMap] at * <;> split) <;> (try grind)
-. unfold contains emptySet at jContained; grind
+. unfold contains emptySet at ⊢ ; simp
 . simp at *; rename_i s; split at s <;> try grind
   subst_vars; simp at *;
-  simp [insertElem, contains, updateMap] at jContained IH
-  cases jContained <;> try grind
-
+  simp [insertElem, contains, updateMap] at ⊢ IH
+  constructor
+  . rename_i cas prom; cases cas <;> try grind
+    rw [(IH sPropNone).right] at *
+    exfalso; grind
+  . exact (IH sPropNone).right
 
 theorem inv4c1Proof (s: System a l p) (i: Fin p):
 systemIsValid s
@@ -51,51 +53,144 @@ induction s0Steps  with
 
 
 
+
+
 --INV4c2
 def inv4c2 (s: System a l p) (i: Fin p) (v: Value):=
 (s.proposers i).propVal = v
--> (∃ j, contains (s.proposers i).propRec j = true
+-> ((∃ j, contains (s.proposers i).propRec j = true
 ∧ Message.Promise (s.proposers i).propId j (some (v, (s.proposers i).accPropId )) ∈ s.network.messages)
 ∧ (∀ j, contains (s.proposers i).propRec j = true
--> (∃ v' id', (Message.Promise (s.proposers i).propId j (some (v', id')) ∈ s.network.messages ∧   id' <= (s.proposers i).accPropId)) ∨ Message.Promise (s.proposers i).propId j none ∈ s.network.messages)
+-> (∃ v' id', (Message.Promise (s.proposers i).propId j (some (v', id')) ∈ s.network.messages ∧   id' <= (s.proposers i).accPropId)) ∨ Message.Promise (s.proposers i).propId j none ∈ s.network.messages)) ∨ (∀ j, contains (s.proposers i).propRec j = true -> Message.Promise (s.proposers i).propId j none ∈ s.network.messages)
+
+
+
+--INV4C21
+def inv4c21 (s1 : System a l p) (i: Fin p) :=
+0 < ((s1.proposers i).accPropId)
+-> ∃ v j, (s1.proposers i).propVal = some v
+∧ (s1.proposers i).propRec j = true
+∧ Message.Promise (s1.proposers i).propId j (some (v, (s1.proposers i).accPropId)) ∈ s1.network.messages
+
+
+theorem inv4c21Proof_ind (s1 s2: System a l p) (i: Fin p):
+step s1 s2
+-> inv4c21 s1 i 
+-> inv4c21 s2 i := by
+simp [inv4c21]; intros step IH sPropTrue
+cases step <;> rename_i stepRule <;> cases stepRule <;> repeat (rename_i stepRule; rcases stepRule) <;> (try simp [updateMap, PropId] at * <;> split) <;> subst_vars <;> (try simp [PropId] at *) <;> (try grind)  <;> (try exact (IH sPropTrue))
+. rename_i prop opt v pid mInN idBound optSome splitX
+  split at splitX <;> try grind
+  . subst splitX; simp [insertElem, updateMap] at *
+    rcases (IH sPropTrue) with ⟨ v1, sPropSome, x, sIsTrue, messInN⟩
+    exists v1; simp [sPropSome]; exists x; simp [sIsTrue, messInN]
+  . clear IH; subst splitX; simp [insertElem, updateMap] at *
+    rename_i bAndOptIsNone; simp [bAndOptIsNone] at optSome
+    rename_i accId
+    subst optSome; simp at *; exists accId; constructor <;> try grind
+. rename_i prop v net k propBound c kNeq
+  rcases c with ⟨ pNat, splitX⟩
+  split at splitX <;> (try rw [splitX]) <;> (try (rw [splitX.left])) <;> (simp [kNeq] at sPropTrue ⊢ ; exact (IH sPropTrue))
+  
+
+
+theorem inv4c21Proof (s: System a l p) (i: Fin p):
+systemIsValid s
+-> inv4c21 s i := by
+intros sIsValid
+have ⟨ s0, s0Inits, s0Steps ⟩ := sIsValid
+induction s0Steps  with
+| refl =>
+  simp [systemInits, proposerInits, networkInits] at s0Inits
+  simp [inv4c21, s0Inits, PropId] at ⊢; 
+| trans s2 s3 s0Steps s2Step IH=>
+  simp [systemIsValid, ] at (IH)
+  have IHApp := IH s0; simp [s0Inits, s0Steps] at IHApp
+  have s2Valid:(systemIsValid s2) := by (simp [systemIsValid]; grind)
+  --have p1:(inv4c1 s2 i):= by {exact (inv4c1Proof s2 i s2Valid)}
+  --have p4:(∀ i v id, inv43 s2 i v id) := by {intros i v id; exact (inv43Proof s2 v i id  s2Valid)}
+  exact (inv4c21Proof_ind s2 s3 i s2Step IHApp )
+
+
+
 
 
 theorem inv4c2Proof_ind (s1 s2: System a l p) (i: Fin p) (v: Value):
 step s1 s2
--> inv4c2 s1 i v
+-> (∀ i v, inv4c2 s1 i v)
 -> (∀ j v id, inv43 s1 j v id)
--> (∀ j, inv4c4 s1 i j)
+-> inv4c21 s1 i
+-> inv4c1 s1 i
 -> inv4c2 s2 i v := by
-simp [inv4c2]; intros step IH i43 i4c4 sPropNone 
-cases step <;> rename_i stepRule <;> cases stepRule <;> repeat (rename_i stepRule; rcases stepRule) <;> (try simp [updateMap] at * <;> split) <;> (try grind) <;> subst_vars
-. rename_i j k prop opt v pid2 mInN  idBound splitX
-  simp at *; split at splitX
-  . subst splitX; simp [contains, insertElem, updateMap] at *
-    constructor <;> try grind
-  . rcases splitX with ⟨ eq1, eq2 ⟩; subst eq1 eq2; simp [contains, insertElem, updateMap] at *
-    constructor <;> try grind
-    subst sPropNone; intros h eq
-    cases eq
-    rename_i k; subst k; left; exists v, pid2; constructor <;> try grind
-    simp [PropId]; rename_i acc
-    sorry
-. simp at *; subst_vars; rename_i v net k retBound
-  split at retBound; try grind
-  . clear IH; rw [retBound]; simp
-. sorry
-
+simp [inv4c2]; intros step IH i43 i4c21 i4c1 sPropNone 
+cases step <;> rename_i stepRule <;> cases stepRule <;> repeat (rename_i stepRule; rcases stepRule) <;> (try simp [updateMap] at * <;> split) <;> (try grind) <;> subst_vars <;> by_cases ((s1.proposers i).propVal = some v) <;> (try grind)
+. rename_i i accId p2 mess opt v2 pid stepRule;
+  simp [updateMap] at *
+  rcases stepRule with ⟨mIsProp, mInN, pidBound, optIsSome, splitX ⟩
+  split at splitX <;> split at sPropNone <;> subst_vars <;> simp [updateMap, insertElem, contains] at * <;> by_cases (opt = none) <;> (try grind) 
+  . left; constructor <;> try grind
+    . have IccBound: (0 < ((s1.proposers i).accPropId)) := by {
+      by_cases ((s1.proposers i).accPropId = 0) <;> try grind
+      . rename_i dEq someNone zeroEq; simp [someNone] at optIsSome dEq
+        rw [zeroEq] at dEq; exfalso; simp at dEq
+      . rename_i a; exact Nat.pos_of_ne_zero a
+      }
+      have ⟨ v, j, r1, r2, r3 ⟩  := i4c21 IccBound
+      grind
+    . intros j jContained; cases jContained <;> try grind
+      . rename_i eq1 eq2; have eq3 := optIsSome eq1
+        subst eq3 eq2; left; exists v2, pid
+        constructor <;> try grind
+        . rename_i contra; simp at contra; exact Nat.le_of_lt contra
+  . left; constructor <;> try grind
+    . rename_i notNone; have someV := optIsSome notNone; subst someV
+      intros j jContained; cases jContained <;> try grind
+      . left; rename_i eq1; subst eq1; exists v2, pid; constructor <;> try grind
+        . simp [PropId]
+      . rename_i jContained;
+        by_cases c: (∃ v, (s1.proposers i).propVal = some v) <;> try grind
+        . have ⟨ v', someExists ⟩  := c
+          rcases (IH i v' someExists) with h1 | h2 <;> try grind
+          . cases (h1.right j jContained) <;> try grind
+            . rename_i eq; rcases eq with ⟨ v2, id2, rest ⟩
+              left; exists v2, id2; constructor <;> try grind
+              rename_i d; exact Nat.le_trans rest.right d.right
+        . have sIsNone:((s1.proposers i).propVal = none) := by cases h : (s1.proposers i).propVal <;> try grind
+          clear c; right; exact (i4c1 sIsNone).left j jContained
+. rename_i prop v2 net j stepRule; simp [updateMap, contains] at *
+  rcases stepRule with ⟨ r1, r2, r3 ⟩ 
+  by_cases (j = i) <;> rename_i eqs <;> simp [eqs] at ⊢ sPropNone r3
+  . subst eqs r2; simp at sPropNone; subst sPropNone
+    split at r3 
+    . rw [r3]; simp at *; rename_i isNone
+      have IHApp := i4c1 isNone; right; exact IHApp.left
+    . rw [r3.left]; simp at *; grind
+  . have IHApp := IH i v sPropNone; split at r3 
+    . rw [r3]; simp; exact IHApp
+    . rw [r3.left]; simp; exact IHApp
 
 theorem inv4c2Proof (s: System a l p) (i: Fin p) (v: Value):
 systemIsValid s
 -> inv4c2 s i v:= by
-intros sIsValid 
-rcases sIsValid with ⟨ s0, s0Inits, s0Steps ⟩
+intros sIsValid
+have ⟨ s0, s0Inits, s0Steps ⟩ := sIsValid
+revert i v
 induction s0Steps  with
 | refl =>
   simp [systemInits, proposerInits, networkInits] at s0Inits
-  simp [inv4c2, s0Inits, ] at ⊢
+  simp [inv4c2, s0Inits] at ⊢
 | trans s2 s3 s0Steps s2Step IH=>
-  sorry
+  intros i v
+  simp [systemIsValid, ] at (IH)
+  have IHApp := IH s0; simp [s0Inits, s0Steps] at IHApp
+  have s2Valid:(systemIsValid s2) := by (simp [systemIsValid]; grind)
+  have p1:(∀ j v id, inv43 s2 j v id):= by {intros v j id; exact (inv43Proof s2 j v id s2Valid)}
+  have p2: inv4c21 s2 i:= by {exact (inv4c21Proof s2 i s2Valid)}
+  have p3: (inv4c1 s2 i):= by {exact (inv4c1Proof s2 i s2Valid)}
+  exact (inv4c2Proof_ind s2 s3 i v s2Step IHApp p1 p2 p3)
+
+
+  
 
 --INV4c3
 def inv4c3 (s: System a l p) (j: Fin p) :=
@@ -133,7 +228,7 @@ Message.Accept (id, v) ∈ s.network.messages
 ∧ (∀ i, contains set i -> ∃ p, Message.Promise id i p ∈ s.network.messages) 
 ∧ ((∀ i, contains set i -> Message.Promise id i none ∈ s.network.messages)
 ∨ (∃ idmax, idmax <= id  ∧ ((∃ i, contains set i ∧ Message.Promise  id i (some (v, idmax)) ∈ s.network.messages)
-∧ (∀ i, contains set i  -> ∃ v' id', Message.Promise id i (some (v', id')) ∈ s.network.messages -> id' <= idmax))))
+∧ (∀ i, contains set i  -> (∃ v' id', Message.Promise id i (some (v', id')) ∈ s.network.messages ∧ id' <= idmax) ∨  Message.Promise id i none ∈ s.network.messages))))
 
 theorem inv4cProof_ind (s1 s2: System a l p) (v: Value) (id: PropId):
 step s1 s2
@@ -156,15 +251,44 @@ cases step <;> rename_i stepRule <;> cases stepRule <;> repeat (rename_i stepRul
   . right; rename_i c; rcases c with ⟨ idMax, idMaxBound, rest ⟩   
     exists idMax; simp [idMaxBound];
     constructor <;> try grind
-    sorry
-. sorry
+    clear IH mNat setContains
+    intros j jContained
+    cases (rest.right j jContained)
+    . left; rename_i d; rcases d with ⟨ v2, id2, mProp ⟩; exists v2, id2; grind
+    . right; grind   
+. simp at *; clear i4c1 i4c2 i4c3 i43
+  have ⟨ set, setCount, setContains ⟩ := IH accInN
+  exists set; simp [setCount]
+  constructor; have c := setContains.left; grind
+  cases setContains.right
+  . left; grind
+  . right; rename_i c; rcases c with ⟨ idMax, idMaxBound, rest ⟩   
+    exists idMax; simp [idMaxBound];
+    constructor <;> try grind
+    clear IH mNat setContains
+    intros j jContained
+    cases (rest.right j jContained)
+    . left; rename_i d; rcases d with ⟨ v2, id2, mProp ⟩; exists v2, id2; grind
+    . right; grind   
 . rename_i prop v2 net j propRecCount pNat splitN; simp at accInN ⊢ 
   split at splitN <;> (try rw [splitN] at accInN ⊢) <;> (try rw [splitN.left] at accInN ⊢) <;> simp at accInN ⊢ <;> cases accInN <;> rename_i accInN <;> (try (exact IH accInN)) <;> exists (s1.proposers j).propRec <;> simp [propRecCount] <;> rename_i eq <;> simp at eq <;> rcases accInN with ⟨ eq1, eq2 ⟩ 
   . have dd := i4c1 j eq
     constructor
-    . intros i iContained; exists none; rw [eq1]; exact (dd i iContained)
-    . left; intros i iContained; rw [eq1]; exact (dd  i iContained)
-  .sorry
+    . intros i iContained; exists none; rw [eq1]; exact (dd.left i iContained)
+    . left; intros i iContained; rw [eq1]; exact (dd.left  i iContained)
+  . clear IH; subst pNat
+    have ⟨ v', rest ⟩:(∃ v , (s1.proposers j).propVal = some v) := by grind
+    have ip4 := i4c2 j v' rest
+    cases ip4 <;> try grind
+    rename_i dd; constructor <;> try grind
+    right; subst eq1 eq2; exists (s1.proposers j).accPropId
+    constructor <;> try grind
+    . exact ( i4c3 j)
+      
+                  
+      
+    
+    
     
     
     
@@ -172,11 +296,19 @@ cases step <;> rename_i stepRule <;> cases stepRule <;> repeat (rename_i stepRul
 theorem inv4cProof (s: System a l p) (v: Value) (id: PropId)  :
 systemIsValid s
 -> inv4c s v id:= by
-intros sIsValid 
-rcases sIsValid with ⟨ s0, s0Inits, s0Steps ⟩
+intros sIsValid
+have ⟨ s0, s0Inits, s0Steps ⟩ := sIsValid
 induction s0Steps  with
 | refl =>
   simp [systemInits, networkInits] at s0Inits
-  simp [inv4c, s0Inits] at ⊢ 
+  simp [inv4c, s0Inits] at ⊢
 | trans s2 s3 s0Steps s2Step IH=>
-  sorry
+  simp [systemIsValid, ] at (IH)
+  have IHApp := IH s0; simp [s0Inits, s0Steps] at IHApp
+  have s2Valid:(systemIsValid s2) := by (simp [systemIsValid]; grind)
+  have p1:(∀ i , inv4c1 s2 i ):= by {intros i; exact (inv4c1Proof s2 i s2Valid)}
+  have p2:(∀ i v, inv4c2 s2 i v) := by {intros i v; exact (inv4c2Proof s2 i v s2Valid)}
+  have p3:(∀ i, inv4c3 s2 i):= by {intros i; exact (inv4c3Proof s2 i s2Valid)}
+  have p4:(∀ i v id, inv43 s2 i v id) := by {intros i v id; exact (inv43Proof s2 v i id  s2Valid)}
+  exact (inv4cProof_ind s2 s3 v id s2Step IHApp p1 p2 p3 p4)
+
